theories/ConcreteRefinement.v
@@ -1,0 +1,93 @@
+From Coq Require Export Morphisms RelationClasses Setoid Program.Equality.
+From ITree Require Export ITree ITreeFacts.
+From Paco Require Import paco.
+From Coq Require Export Eqdep EqdepFacts.
+Require Import Lia.
+Require Export Refinement ConvergentRefinement.
+
+Variant no_eventsF {E R} (F : itree E R -> Prop) : itree' E R -> Prop :=
+  | no_events_Ret r : no_eventsF F (RetF r)
+  | no_events_Tau t : F t -> no_eventsF F (TauF t).
+
+Definition no_events_ {E R} F (t : itree E R) : Prop :=
+  no_eventsF F (observe t).
+
+
+Lemma monot_no_events E R : monotone1 (@no_events_ E R).
+Proof.
+  red. unfold no_events_. intros.
+  induction IN; constructor; auto.
+Qed.
+
+Hint Resolve monot_no_events : paco.
+
+Definition no_events {E R } : itree E R -> Prop := paco1 no_events_ bot1.
+
+Global Instance proper_no_events_eutt {E R} : Proper (eutt eq ==> flip impl) (@no_events E R).
+Proof.
+  pcofix CIH.
+  intros t1 t2 Ht Hno. pstep. red.
+  punfold Hno. red in Hno. punfold Ht. red in Ht.
+  hinduction Ht before r; intros.
+  - constructor.
+  - constructor. inv Hno. pclearbot. right. eauto.
+  - inv Hno.
+  - constructor. left. pstep. eapply IHHt; eauto.
+  - inv Hno. pclearbot. eapply IHHt; eauto. pstep_reverse.
+Qed.
+
+Global Instance proper_isConcrete_eutt {E R} : Proper (eutt eq ==> flip impl) (@isConcrete E R).
+Proof.
+  pcofix CIH.
+  intros t1 t2 Ht Hcon. pstep. red.
+  punfold Hcon. red in Hcon. punfold Ht. red in Ht.
+  hinduction Ht before r; intros.
+  - constructor.
+  - inv Hcon. pclearbot. constructor. eauto.
+  - inv Hcon. inj_existT. subst. pclearbot. constructor.
+    right. eapply CIH; eauto. apply REL. apply H0.
+  - constructor. left. pstep. eapply IHHt; eauto.
+  - inv Hcon. pclearbot. eapply IHHt; auto. pstep_reverse.
+Qed.
+(*should it be refines or padded refines? lifting to padded_refines is actually simple 
+   because each other predicate respects eutt *)
+Theorem concrete_conv_ref_to_no_ev E1 E2 R1 R2 RE REAns RR :
+  forall (t : itree_spec E1 R1) (phi : itree_spec E2 R2), isConcrete t -> conv_ref phi ->
+                                                     refines RE REAns RR t phi ->
+                                                     no_events t.
+Proof.
+  pcofix CIH.
+  intros t phi Hcon Hconv Href.
+  punfold Hcon. red in Hcon.
+  punfold Hconv. red in Hconv.
+  punfold Href. red in Href.
+  pstep. red. hinduction Href before r; intros.
+  - constructor.
+  - constructor. right. inv Hcon. inv Hconv. pclearbot. eauto.
+  - inv Hcon. pclearbot. constructor. right. eapply CIH; eauto.
+    Unshelve. 3 : (apply (go ophi)). pstep. auto. pstep. auto.
+  - inv Hconv. pclearbot. eapply IHHref; eauto. pstep_reverse.
+  - inv Hconv.
+  - inv Hconv. inj_existT. subst. pclearbot. eapply H0; eauto.
+    pstep_reverse.
+  - inv Hcon.
+  - inv Hconv. inj_existT. subst. pclearbot. eapply IHHref; eauto. pstep_reverse.
+  - inv Hcon.
+    Unshelve. auto.
+Qed.
+
+Theorem concrete_conv_ref_padded_to_no_ev E1 E2 R1 R2 RE REAns RR :
+  forall (t : itree_spec E1 R1) (phi : itree_spec E2 R2), isConcrete t -> conv_ref phi ->
+                                                     padded_refines RE REAns RR t phi ->
+                                                     no_events t.
+Proof.
+  intros t phi Hcon Hconv Href. red in Href. rewrite  pad_eutt.
+  eapply concrete_conv_ref_to_no_ev with (phi := pad phi); eauto.
+  - rewrite <- pad_eutt. auto.
+  - rewrite <- pad_eutt. auto.
+Qed.
+
+(*relies on lem*)
+Theorem no_ev_to_dec E R : forall (t : itree E R), no_events t -> 
+                                              (exists r, t ≈ Ret r) \/ t ≈ ITree.spin.
+Admitted.
